theories/utils/bitblast.v
@@ -540,37 +540,3 @@ Tactic Notation "bitblast" ident(H) "with" constr(i) "as" ident(H') :=
   end; bitblast H'.
 Tactic Notation "bitblast" ident(H) "with" constr(i) :=
   let H' := fresh "H" in bitblast H with i as H'.
-
-(* TODO move in switcher_preamble *)
-Definition encode_entry_point (nargs entry_point_offset : Z) : Z :=
-  let args := Z.land nargs 7 in
-  let off := Z.shiftl entry_point_offset 3 in
-  (Z.lor off args).
-
-Definition decode_entry_point (entry_point : Z) : (Z * Z) :=
-  ( Z.land entry_point 7, Z.shiftr entry_point 3).
-
-Lemma encode_entry_point_eq_nargs nargs off_entry :
-  (0 ≤ nargs ≤ 7)%Z -> ( (Z.land (encode_entry_point nargs off_entry) 7)) = nargs.
-Proof.
-  intros.
-  rewrite /encode_entry_point.
-  bitblast.
-  destruct (decide (nargs = 0)); simplify_eq; first bitblast.
-  destruct (decide (nargs = 1)); simplify_eq; first bitblast.
-  destruct (decide (nargs = 2)); simplify_eq; first bitblast.
-  destruct (decide (nargs = 3)); simplify_eq; first bitblast.
-  destruct (decide (nargs = 4)); simplify_eq; first bitblast.
-  destruct (decide (nargs = 5)); simplify_eq; first bitblast.
-  destruct (decide (nargs = 6)); simplify_eq; first bitblast.
-  destruct (decide (nargs = 7)); simplify_eq; first bitblast.
-  lia.
-Qed.
-
-Lemma encode_entry_point_eq_off nargs off_entry :
-  ( (encode_entry_point nargs off_entry ≫ 3)) = off_entry.
-Proof.
-  intros.
-  rewrite /encode_entry_point.
-  bitblast.
-Qed.
