theories/utils/iris_extra.v
@@ -166,6 +166,21 @@ Proof.
   rewrite (delete_take_drop b). rewrite (delete_take_drop a). iFrame.
 Qed.
 
+Lemma big_sepL_elem_of_extract {Σ : gFunctors} { A : Type } (P Q : A -> iProp Σ) (a : A) (l : list A) :
+  a ∈ l ->
+  NoDup l ->
+  (∀ a, P a -∗ Q a) -∗
+  ([∗ list] a ∈ l, P a) -∗
+  ∃ l', ⌜ l ≡ₚ a::l' ⌝ ∗ ([∗ list] a ∈ l', P a) ∗ (Q a).
+Proof.
+  iIntros (Ha_in Hnodup) "Himpl Hl".
+  apply elem_of_Permutation in Ha_in as [l' Hl'].
+  iExists l'; iFrame "%".
+  iEval (setoid_rewrite Hl') in "Hl".
+  iDestruct "Hl" as "[Ha $]".
+  by iApply "Himpl".
+Qed.
+
 Lemma big_sepL2_close_l {Σ : gFunctors} {A B : Type} (i : nat) (ai : A) (bi : B) (a : list A) (b : list B) (φ : A -> B -> iProp Σ) :
   length a = length b ->
   a !! i = Some ai ->
